passing chacha-curve-poly-aes test vectors

spec-checker-ocaml/fstar-compiler/specs/tests/poly1305_test.ml
@@ -1,0 +1,19 @@
+open Yojson.Basic.Util
+open Testutil
+   
+let main () =
+  let json = Yojson.Basic.from_file "../../../tests/test_vectors/poly1305_test_vectors.json" in
+  let jsonl = Yojson.Basic.Util.to_list json in
+  List.iteri (fun i j ->
+      let key = read_bytes j "key" in
+      let input = read_bytes j "input" in
+      let output = read_bytes j "tag" in
+      let computed = Poly1305.poly1305_mac input key in
+      if output = computed then Printf.printf "Poly1305 Test %d passed.\n" i
+      else (Printf.printf "Poly1305 Test %d failed.\n" i;
+            Printf.printf "expected ciphertext: %s\n" (hex_of_bytes output);
+            Printf.printf "computed ciphertext: %s\n" (hex_of_bytes computed));
+      ()) jsonl;
+  ()
+
+let _ = main()
