spec-checker-ocaml/fstar-compiler/specs/tests/testutil.ml
@@ -1,0 +1,49 @@
+open Yojson.Basic
+open Yojson.Basic.Util
+
+let digit_to_int c = match c with
+  | '0'..'9' -> Char.code c - Char.code '0'
+  | 'a'..'f' -> 10 + Char.code c - Char.code 'a'
+  | 'A'..'F' -> 10 + Char.code c - Char.code 'A'
+  | _ -> failwith "hex_to_char: invalid hex digit"
+
+let hex_to_int a b =
+  ((digit_to_int a) lsl 4 + digit_to_int b)
+
+let int_to_hex n =
+  let digits = "0123456789abcdef" in
+  digits.[n lsr 4], digits.[n land 0x0f]
+
+let int_list_of_hex s =
+  let n = String.length s in
+  if n mod 2 <> 0 then
+     failwith "string_of_hex: invalid length"
+  else
+    let rec aux i =
+      if i >= n then []
+      else (
+       (hex_to_int s.[i] s.[i+1]) :: aux (i+2)
+      )
+    in
+    aux 0
+let bytes_of_hex s : FStar_UInt8.t Lib_Sequence.seq  = (int_list_of_hex s)
+
+let rec hex_of_int_list l =
+  match l with
+  | [] -> ""
+  | h::t -> let a,b = int_to_hex h in
+            Char.escaped a ^ Char.escaped b ^ hex_of_int_list t
+let hex_of_bytes b = hex_of_int_list b
+
+let uint32_of_int_list l =
+  match l with
+  | [a;b;c;d] -> a lsl 24 + b lsl 16 + c lsl 8 + d
+  | _ -> failwith "uint32_of_int_list: invalid length"
+
+let uint32_of_hex h = uint32_of_int_list (int_list_of_hex h)
+
+let read_bytes j n = j |> member n |> to_string |> bytes_of_hex
+let read_uint32 j n = j |> member n |> to_string |> uint32_of_hex
+let read_int j n = j |> member n |> to_int
+let read_bool j n = j |> member n |> to_bool
+                                                     
