spec-checker-ocaml/fstar-compiler/specs/speclib.fst
@@ -3,195 +3,203 @@ open Lib.IntTypes
 open Lib.Sequence
 open Lib.ByteSequence
 
-type nat_t = nat
-type pos_t = pos
+inline_for_extraction type nat_t = nat
+inline_for_extraction type pos_t = pos
 
 type numeric = 
   | Word of inttype
   | Int 
 
-let numeric_t (n:numeric) = 
+inline_for_extraction let numeric_t (n:numeric) = 
   match n with
   | Word i -> uint_t i
   | Int -> int
 
-let zero (n:numeric) : numeric_t n = 
+inline_for_extraction let zero (n:numeric) : numeric_t n = 
   match n with
   | Word t -> nat_to_uint #t 0
   | Int -> 0
 
-let one (n:numeric) : numeric_t n = 
+inline_for_extraction let one (n:numeric) : numeric_t n = 
   match n with
   | Word t -> nat_to_uint #t 1
   | Int -> 1
 
-let bitvector (n:numeric) = 
+inline_for_extraction let bitvector (n:numeric) = 
   match n with
   | Word i -> machineint i
   | Int -> False
 
-let comparable (n:numeric) = 
+inline_for_extraction let comparable (n:numeric) = 
   match n with
   | Word SIZE -> True
   | Word (NATm _) -> True
   | Int -> True
   | _ -> False
 
-let divisible (n:numeric) = 
+inline_for_extraction let divisible (n:numeric) = 
   match n with
   | Word SIZE -> True
   | Word (NATm _) -> True
   | Int -> True
   | _ -> False
 
-let shiftval (n:numeric{bitvector n}) =
+inline_for_extraction let shiftval (n:numeric{bitvector n}) =
   match n with
   | Word t -> n:nat{n < bits t} //shiftval t
 
-let rotval (n:numeric{bitvector n}) =
+inline_for_extraction let rotval (n:numeric{bitvector n}) =
   match n with
   | Word t -> n:nat{n > 0 /\ n < bits t} //rotval t
 
-let (+.) (#n:numeric) (a:numeric_t n) (b:numeric_t n) : numeric_t n = 
+inline_for_extraction let (+.) (#n:numeric) (a:numeric_t n) (b:numeric_t n) : numeric_t n = 
   match n with
   | Word t -> (a <: uint_t t) +. b
   | Int -> a + b
 
-let (-.) (#n:numeric) (a:numeric_t n) (b:numeric_t n) : numeric_t n = 
+inline_for_extraction let (-.) (#n:numeric) (a:numeric_t n) (b:numeric_t n) : numeric_t n = 
   match n with
   | Word t -> (a <: uint_t t) -. b
   | Int -> a - b
 
-let ( *. ) (#n:numeric{n <> Word U128}) (a:numeric_t n) (b:numeric_t n) : numeric_t n = 
+inline_for_extraction let ( *. ) (#n:numeric{n <> Word U128}) (a:numeric_t n) (b:numeric_t n) : numeric_t n = 
   match n with
   | Word t -> (a <: uint_t t) *. b
   | Int -> a `op_Multiply` b
 
-let (/.) (#n:numeric{divisible n}) (a:numeric_t n) (b:numeric_t n) : numeric_t n = 
+inline_for_extraction let (/.) (#n:numeric{divisible n}) (a:numeric_t n) (b:numeric_t n) : numeric_t n = 
   match n with
   | Word t -> (a <: uint_t t) /. b
   | Int -> a / b
 
-let (%.) (#n:numeric{divisible n}) (a:numeric_t n) (b:numeric_t n) : numeric_t n = 
+inline_for_extraction let (%.) (#n:numeric{divisible n}) (a:numeric_t n) (b:numeric_t n) : numeric_t n = 
   match n with
   | Word t -> (a <: uint_t t) %. b
   | Int -> a % b
 
 
-let ( <<. ) (#n:numeric{bitvector n}) (a:numeric_t n) (b:shiftval n) : numeric_t n = 
+inline_for_extraction let ( <<. ) (#n:numeric{bitvector n}) (a:numeric_t n) (b:shiftval n) : numeric_t n = 
   match n with
   | Word t -> (a <: uint_t t) <<. u32 b
 
-let ( >>. ) (#n:numeric{bitvector n}) (a:numeric_t n) (b:shiftval n) : numeric_t n = 
+inline_for_extraction let ( >>. ) (#n:numeric{bitvector n}) (a:numeric_t n) (b:shiftval n) : numeric_t n = 
   match n with
   | Word t -> (a <: uint_t t) >>. u32 b
 
-let ( &. ) (#n:numeric{bitvector n}) (a:numeric_t n) (b:numeric_t n) : numeric_t n = 
+inline_for_extraction let ( &. ) (#n:numeric{bitvector n}) (a:numeric_t n) (b:numeric_t n) : numeric_t n = 
   match n with
   | Word t -> (a <: uint_t t) &. b
 
-let ( |. ) (#n:numeric{bitvector n}) (a:numeric_t n) (b:numeric_t n) : numeric_t n = 
+inline_for_extraction let ( |. ) (#n:numeric{bitvector n}) (a:numeric_t n) (b:numeric_t n) : numeric_t n = 
   match n with
   | Word t -> (a <: uint_t t) |. b
 
-let ( ^. ) (#n:numeric{bitvector n}) (a:numeric_t n) (b:numeric_t n) : numeric_t n = 
+inline_for_extraction let ( ^. ) (#n:numeric{bitvector n}) (a:numeric_t n) (b:numeric_t n) : numeric_t n = 
   match n with
   | Word t -> (a <: uint_t t) ^. b
 
-let ( <=. ) (#n:numeric{comparable n}) (a:numeric_t n) (b:numeric_t n) : bool = 
+inline_for_extraction let ( <=. ) (#n:numeric{comparable n}) (a:numeric_t n) (b:numeric_t n) : bool = 
   match n with
   | Word t -> (a <: uint_t t) <=. b
   | Int -> a <= b
 
-let ( =. ) (#n:numeric{comparable n}) (a:numeric_t n) (b:numeric_t n) : bool = 
+inline_for_extraction let ( =. ) (#n:numeric{comparable n}) (a:numeric_t n) (b:numeric_t n) : bool = 
   match n with
   | Word t -> (a <: uint_t t) =. b
   | Int -> a = b
 
-let ( >. ) (#n:numeric{comparable n}) (a:numeric_t n) (b:numeric_t n) : bool = 
+inline_for_extraction let ( >. ) (#n:numeric{comparable n}) (a:numeric_t n) (b:numeric_t n) : bool = 
   match n with
   | Word t -> (a <: uint_t t) >. b
   | Int -> a > b
 
-let rec exp  (#n:numeric{n <> Word U128}) (x:numeric_t n) (y:nat) : numeric_t n = 
-    if y = 0 then one n
-    else x *. (exp x (y-1))
+inline_for_extraction let rec exp  (#n:numeric{n <> Word U128}) (x:numeric_t n) (y:nat) : numeric_t n = 
+    if y = 0 then one n 
+    else if y = 1 then x
+    else 
+      let xn = exp x (y / 2) in
+      let xn2 = xn *. xn in
+      if y % 2 = 0 then xn2
+      else xn2 *. x
 
-let ( **. ) (#n:numeric{n <> Word U128}) (x:numeric_t n) (y:nat) : numeric_t n = 
+inline_for_extraction let ( **. ) (#n:numeric{n <> Word U128}) (x:numeric_t n) (y:nat) : numeric_t n = 
     if n = Int && x = 2 then pow2 y
     else exp #n x y
 
-let natmod_t (n:pos) = numeric_t (Word (NATm n))
-let natmod n p : natmod_t p = n % p
-let natmod_to_nat (#m:pos) (a:natmod_t m) : x:nat{x < m}  = a
-let natmod_to_int (#m:pos) (a:natmod_t m) : x:nat{x < m}  = a
+inline_for_extraction let natmod_t (n:pos) = numeric_t (Word (NATm n))
+inline_for_extraction let natmod n p : natmod_t p = n % p
+inline_for_extraction let natmod_to_nat (#m:pos) (a:natmod_t m) : x:nat{x < m}  = a
+inline_for_extraction let natmod_to_int (#m:pos) (a:natmod_t m) : x:nat{x < m}  = a
 
-let uintn_t (n:nat) = numeric_t (Word (NATm (pow2 n)))
-let uint32_t = numeric_t (Word U32)
-let bit_t = numeric_t (Word (NATm 2))
-let uint8_t = numeric_t (Word U8)
-let uint128_t = numeric_t (Word U128)
-let uint64_t = numeric_t (Word U64)
+inline_for_extraction let uintn_t (n:nat) = numeric_t (Word (NATm (pow2 n)))
+inline_for_extraction let uint32_t = numeric_t (Word U32)
+inline_for_extraction let bit_t = numeric_t (Word (NATm 2))
+inline_for_extraction let uint8_t = numeric_t (Word U8)
+inline_for_extraction let uint128_t = numeric_t (Word U128)
+inline_for_extraction let uint64_t = numeric_t (Word U64)
 
-let uintn n p : uintn_t p = natmod n (pow2 p)
-let bit x : bit_t = modulo x 2
-let uint8 x : uint8_t = u8 x
-let uint32 x : uint32_t = u32 x
-let uint128 x : uint128_t = u128 x
+inline_for_extraction let uintn n p : uintn_t p = natmod n (pow2 p)
+inline_for_extraction let bit x : bit_t = modulo x 2
+inline_for_extraction let uint8 x : uint8_t = u8 x
+inline_for_extraction let uint32 x : uint32_t = u32 x
+inline_for_extraction let uint128 x : uint128_t = u128 x
 
-let uintn_to_nat #t (a:uint_t t) : nat = Lib.RawIntTypes.uint_to_nat a
-let uintn_to_int #t (a:uint_t t) : nat = Lib.RawIntTypes.uint_to_nat a
-let uintn_get_bit #b (x:uintn_t b) (i:nat) : bit_t  = bit (((uintn_to_nat x) / pow2 i) % 2)
-let uintn_rotate_left (#t:m_inttype) (a:uint_t t) b = a <<<. (u32 b)
-let uintn_rotate_right (#t:m_inttype) (a:uint_t t) b = a >>>. (u32 b)
+inline_for_extraction let uintn_to_nat #t (a:uint_t t) : nat = 
+		      match t with 
+		      | NATm m -> a 
+		      | _ -> Lib.RawIntTypes.uint_to_nat a
+inline_for_extraction let uintn_to_int #t (a:uint_t t) : nat = uintn_to_nat #t a
+inline_for_extraction let uintn_get_bit #b (x:uintn_t b) (i:nat) : bit_t  = bit (((uintn_to_nat #(NATm (pow2 b)) x) / pow2 i) % 2)
+inline_for_extraction let uintn_rotate_left (#t:m_inttype) (a:uint_t t) b = a <<<. (u32 b)
+inline_for_extraction let uintn_rotate_right (#t:m_inttype) (a:uint_t t) b = a >>>. (u32 b)
 
 type result_t (t:Type0) = 
   | Retval of t
   | Error of string
-let result_retval #t (x:t) : result_t t = Retval x
-let result_error #t (x:string) : result_t t = Error x
+inline_for_extraction let result_retval #t (x:t) : result_t t = Retval x
+inline_for_extraction let result_error #t (x:string) : result_t t = Error x
 
-let range_t min max = n:nat{n >= min /\ n < max}
+inline_for_extraction let range_t min max = n:nat{n >= min /\ n < max}
 unfold let range i = i
-let repeati = repeati
+inline_for_extraction let repeati = repeati
 
-let array_t t len = lseq t len
-let vlarray_t t = seq t
-let array x = x
-let array_length a = length a
-let array_copy #a #l (x:array_t a l) : array_t a l = x
-let op_String_Access #a #len = index #a #len
-let op_String_Assignment #a #len = upd #a #len
-let array_createL l = createL l
-let array_create x y = create x y
-let array_slice #l (x:lseq 'a l) y z = slice x y z
-let array_update_slice #l (x:lseq 'a l) y z w = update_slice x y z w
-val array_split_blocks: #a:Type -> s:seq a -> bs:size_nat{bs > 0} -> (bl:lseq (lseq a bs) (length s / bs) * l:lseq a (length s % bs))
-let array_split_blocks #a s bs = 
+inline_for_extraction let array_t t len = lseq t len
+inline_for_extraction let vlarray_t t = seq t
+inline_for_extraction let array x = x
+inline_for_extraction let array_length a = length a
+inline_for_extraction let array_copy #a #l (x:array_t a l) : array_t a l = x
+inline_for_extraction let op_String_Access #a #len = index #a #len
+inline_for_extraction let op_String_Assignment #a #len = upd #a #len
+inline_for_extraction let array_createL l = createL l
+inline_for_extraction let array_create x y = create x y
+inline_for_extraction let array_slice #l (x:lseq 'a l) y z = slice x y z
+inline_for_extraction let array_update_slice #l (x:lseq 'a l) y z w = update_slice x y z w
+inline_for_extraction val array_split_blocks: #a:Type -> s:seq a -> bs:size_nat{bs > 0} -> (bl:lseq (lseq a bs) (length s / bs) * l:lseq a (length s % bs))
+inline_for_extraction let array_split_blocks #a s bs = 
     let nblocks = length s / bs in
     let rem = length s % bs in
     let blocks = create nblocks (create bs (u8 0)) in
     repeati nblocks (fun i blocks -> blocks.[i] <- sub (to_lseq s) (i `op_Multiply` bs) bs) blocks,
     sub (to_lseq s) (length s - rem) rem 
     
-val array_concat_blocks: #a:Type -> #n:size_nat -> #bs:size_nat{bs > 0} -> bl:lseq (lseq a bs) n -> l:seq a -> r:lseq a (n `op_Multiply` bs + length l)
-let array_concat_blocks #a #n #bs bl l = 
+inline_for_extraction val array_concat_blocks: #a:Type -> #n:size_nat -> #bs:size_nat{bs > 0} -> bl:lseq (lseq a bs) n -> l:seq a -> r:lseq a (n `op_Multiply` bs + length l)
+inline_for_extraction let array_concat_blocks #a #n #bs bl l = 
     let msg = create (n `op_Multiply` bs + length l) (u8 0) in
     let msg = repeati n (fun i msg -> update_sub msg (i `op_Multiply` bs) bs bl.[i]) msg in
     update_sub msg (n `op_Multiply` bs) (length l) l
 
 
-let bytes_t len = lbytes len
-let vlbytes_t = bytes
-let bytes x = x
-let bytes_copy x = x
-let bytes_length x = length x
-let bytes_to_uint32s_le #l (b:lbytes (l `op_Multiply` 4)) = uints_from_bytes_le #U32 #l b
-let bytes_from_uint32s_le #l (b:lseq uint32_t l) = uints_to_bytes_le #U32 b 
-let bytes_to_nat_le #l (b:lbytes l) = nat_from_bytes_le #l b
-let bytes_from_nat_le n l = nat_to_bytes_le l n 
-let bytes_to_uint128_le #l (b:lbytes l) = uint_from_bytes_le #U128 b
-let bytes_from_uint128_le n = uint_to_bytes_le #U128 n
-let bytes_to_uint32_be #l (b:lbytes l) = uint_from_bytes_be #U32 b
-let bytes_from_uint32_be n = uint_to_bytes_be #U32 n
+inline_for_extraction let bytes_t len = lbytes len
+inline_for_extraction let vlbytes_t = bytes
+inline_for_extraction let bytes x = x
+inline_for_extraction let bytes_copy x = x
+inline_for_extraction let bytes_length x = length x
+inline_for_extraction let bytes_to_uint32s_le #l (b:lbytes (l `op_Multiply` 4)) = uints_from_bytes_le #U32 #l b
+inline_for_extraction let bytes_from_uint32s_le #l (b:lseq uint32_t l) = uints_to_bytes_le #U32 b 
+inline_for_extraction let bytes_to_nat_le #l (b:lbytes l) = nat_from_bytes_le #l b
+inline_for_extraction let bytes_from_nat_le n l = nat_to_bytes_le l n 
+inline_for_extraction let bytes_to_uint128_le #l (b:lbytes l) = uint_from_bytes_le #U128 b
+inline_for_extraction let bytes_from_uint128_le n = uint_to_bytes_le #U128 n
+inline_for_extraction let bytes_to_uint32_be #l (b:lbytes l) = uint_from_bytes_be #U32 b
+inline_for_extraction let bytes_from_uint32_be n = uint_to_bytes_be #U32 n
 
